Evaluator proved correct

src/vminus/OpSemEval.v
@@ -22,38 +22,132 @@ Module MakeEval (Import Cfg:CFG).
 Module SS := Make Cfg. 
 Import SS.
 
-(** *** Small-step, executable operational semantics *)
 
-Fixpoint step (g : Cfg.t) (s : state) : err state :=
-  let 'mkst mem pc loc ppc ploc := s in
-  match (fetch g pc) with
-  | Some (uid, cmd_bop bop v1 v2) =>    
-    let result := eval_bop loc bop v1 v2 in
-    match result with
-    | Some n => inr (mkst mem (incr_pc pc) (update loc uid (Some n)) ppc ploc)
-    | None => inl "cannot evalute binop command"%string
-    end 
-  | Some (uid, cmd_phi pas) =>
-    let result := eval_phi ploc (lbl_of ppc) pas in
-    match result with
-    | Some n => inr (mkst mem (incr_pc pc) (update loc uid (Some n)) ppc ploc)
-    | None => inl "cannot evaluate phi"%string
-    end
-  | Some (uid, cmd_tmn tmn) =>
-    let result := eval_tmn loc tmn in
-    match result with
-    | Some l' => inr (mkst mem (block_entry l') loc pc loc)
-    | None => inl "cannot evaluate terminator"%string
-    end
-  | Some (uid, cmd_load addr) =>
-    inr (mkst mem (incr_pc pc) (update loc uid (Some (mem addr))) ppc ploc)
-  | Some (uid, cmd_store addr v) => 
-    let result := eval_val loc v in
-    match result with
-    | Some n => inr (mkst (Memory.update mem addr n) (incr_pc pc) loc pc ploc)
-    | None => inl "cannot evaluate address to store to"%string
-    end
-  | None => inl "no instruction fetched"%string
-  end.
+Module Evaluator.
+  (** *** Small-step, executable operational semantics *)
 
+  Fixpoint eval_step (g : Cfg.t) (s : state) : err state :=
+    let 'mkst mem pc loc ppc ploc := s in
+    match (fetch g pc) with
+    | Some (uid, cmd_bop bop v1 v2) =>    
+      let result := eval_bop loc bop v1 v2 in
+      match result with
+      | Some n => inr (mkst mem (incr_pc pc) (update loc uid (Some n)) ppc ploc)
+      | None => inl "cannot evalute binop command"%string
+      end 
+    | Some (uid, cmd_phi pas) =>
+      let result := eval_phi ploc (lbl_of ppc) pas in
+      match result with
+      | Some n => inr (mkst mem (incr_pc pc) (update loc uid (Some n)) ppc ploc)
+      | None => inl "cannot evaluate phi"%string
+      end
+    | Some (uid, cmd_tmn tmn) =>
+      let result := eval_tmn loc tmn in
+      match result with
+      | Some l' => inr (mkst mem (block_entry l') loc pc loc)
+      | None => inl "cannot evaluate terminator"%string
+      end
+    | Some (uid, cmd_load addr) =>
+      inr (mkst mem (incr_pc pc) (update loc uid (Some (mem addr))) ppc ploc)
+    | Some (uid, cmd_store addr v) => 
+      let result := eval_val loc v in
+      match result with
+      (* | Some n => BUG HERE
+           inr (mkst (Memory.update mem addr n) (incr_pc pc) loc pc ploc) *)
+      | Some n => inr (mkst (Memory.update mem addr n) (incr_pc pc) loc ppc ploc)
+      | None => inl "cannot evaluate address to store to"%string
+      end
+    | None => inl "no instruction fetched"%string
+    end.
+
+End Evaluator.
+
+Module EvaluatorCorrect.
+  Import Evaluator.
+
+  Ltac eval_step_with_step next_state constructor_rule
+       cfg_well_formed fetched :=
+    match goal with
+    | H: match ?X with
+         | Some _ => _
+         | None => _ end = inr next_state |-
+      step ?cfg ?curr_state next_state =>
+      
+      destruct X eqn:Heval; 
+      inversion H;
+      eapply constructor_rule;
+      try rewrite insn_at_pc_fetch;
+      try apply fetched;
+      try apply cfg_well_formed;
+      rewrite Heval;
+      reflexivity
+    | H : _ = inr next_state |-
+      step ?cfg ?curr_state next_state =>
+      
+      inversion H;
+      eapply constructor_rule;
+      try rewrite insn_at_pc_fetch;
+      try apply fetched;
+      try apply cfg_well_formed;
+      reflexivity
+    end.
+
+  Ltac cases_on_eval_step_in_goal eval_insn :=
+    match goal with
+    | |- match ?X with
+        | Some _ => _
+        | None => _ end = inr _  =>
+      destruct X;
+      inversion eval_insn;
+      reflexivity
+    end.
+
+  Lemma evaluator_sound: forall g s s',
+      wf_cfg g -> eval_step g s = inr s' -> step g s s'.
+  Proof.
+    intros g s s' wf_g.
+    destruct s as [mem curr_pc curr_loc previous_pc previous_loc];
+      simpl.
+    destruct (fetch g curr_pc) as 
+        [[uid [bop v1 v2 | pas | term | addr | addr v]] | ] eqn:fetched;
+      intros H;
+      [eval_step_with_step s' step_bop wf_g fetched |
+       eval_step_with_step s' step_phi wf_g fetched |
+       eval_step_with_step s' step_tmn wf_g fetched |
+       eval_step_with_step s' step_load wf_g fetched |
+       eval_step_with_step s' step_store wf_g fetched | idtac].
+    inversion H.
+  Qed.
+    
+  Lemma evaluator_complete: forall g s s',
+      wf_cfg g -> step g s s' -> eval_step g s = inr s'.
+  Proof.
+    intros g s s' wf_g step_rel.
+    Print step.
+    inversion step_rel as
+        [mem pc loc bop v1 v2 uid n ppc ploc insn_at_pc_is eval_insn_ok s_eq s'_eq |
+         mem pc loc pas uid n ppc ploc insn_at_pc_is eval_insn_ok s_eq s'_eq |
+         mem pc label loc term uid ppc ploc insn_at_pc_is eval_insn_ok s_eq s'_eq |
+         mem pc loc uid addr ppc ploc insn_at_pc_is eval_insn_ok s'_eq |
+         mem pc loc uid addr v n ppc ploc insn_at_pc_is eval_insn_ok s_eq s'_eq];
+      simpl;
+      destruct (fetch g pc) as [[curr_uid curr_cmd] | ] eqn:fetched; 
+      rewrite insn_at_pc_fetch in insn_at_pc_is; try apply wf_g;
+        rewrite insn_at_pc_is in fetched;
+        inversion fetched;
+        try cases_on_eval_step_in_goal eval_insn_ok.
+    reflexivity.
+  Qed.
+
+  Theorem evaluator_correct: forall g s s',
+      wf_cfg g -> eval_step g s = inr s' <-> step g s s'.
+  Proof.
+    intros g s s' wf_g; split;
+      revert g s s' wf_g.
+    apply evaluator_sound.
+    apply evaluator_complete.
+  Qed.
+
+End EvaluatorCorrect.
+    
 End MakeEval.
